

# 04: Matrix Multiplication as a Composition of Transformations

**Chapter Goal:** To understand that multiplying two matrices is the algebraic representation of a geometric action: **composing** or applying two [transformations](#) one after the other.

---

## 1. Core Idea: Applying Transformations Sequentially

- **Problem:** What happens if we apply one transformation ( $A_1$ ), and then apply another transformation ( $A_2$ ) to the result?
  - **Composition:** The action of "applying one transformation then another" is called a **Composition**.
  - **Final Result:** The outcome of this entire process (from start to finish) is a **single, new transformation** that encapsulates both actions.
- 

## 2. Two Ways of Thinking, One Answer

There are two ways to find the matrix of this combined transformation:

### Method #1: Geometric (Following the Basis Vectors)

1. Start with the standard basis vectors  $\hat{i}$  and  $\hat{j}$ .
2. Apply the **first transformation** ( $A_1$ ) to  $\hat{i}$  and  $\hat{j}$  to get  $\hat{i}'$  and  $\hat{j}'$ .
3. **NOW**, apply the **second transformation** ( $A_2$ ) to the results from step 2 ( $\hat{i}'$  and  $\hat{j}'$ ) to get the final positions  $\hat{i}''$  and  $\hat{j}''$ .
4. The combined matrix ( $A_2A_1$ ) is the matrix whose columns are the **FINAL** positions of the basis vectors, namely  $\hat{i}''$  and  $\hat{j}''$ .

### Method #2: Algebraic (Matrix Multiplication)

1. The combined matrix ( $A_2A_1$ ) can be calculated directly by multiplying matrix  $A_2$  by matrix  $A_1$ .
2. **Reading Rule:** Just like function composition  $g(f(x))$ , we read it from **right to left**.  $A_2A_1$  means "**apply**  $A_1$  **first**, **then apply**  $A_2$ ".
3. **Calculation Rule:** "Row times column". To find the entry in row  $i$ , column  $j$  of the resulting matrix, you multiply row  $i$  of the left matrix with column  $j$  of the right matrix.

The video demonstrates that both of these methods (Geometric and Algebraic) will produce the **exact same final matrix**.

---

### 3. Important Properties of Matrix Multiplication

- **NOT Commutative:**

|  $A_1 A_2 \neq A_2 A_1$

- **Meaning:** The **order** of transformations matters GREATLY.
- **Visual Intuition:** "Rotating by  $90^\circ$  then reflecting vertically" gives a **DIFFERENT** final result than "Reflecting vertically first, then rotating by  $90^\circ$ ". The video proves this visually and with matrix calculations.
- **Associative:**

|  $A_3(A_2 A_1) = (A_3 A_2)A_1$

- **Meaning:** The way we **group** the multiplications doesn't matter, as long as the order remains the same.
- **Visual Intuition:** "Apply  $A_1$ , then  $A_2$ , then  $A_3$ " will always be the same, regardless of whether you think of it as  $(A_3(A_2 A_1))$  or  $((A_3 A_2)A_1)$ . The sequence of actions remains  $A_1 \rightarrow A_2 \rightarrow A_3$ .

---

### 4. Key Message

- [Perkalian Matriks](#) is not just an arbitrary operation on numbers.
- It is the algebraic representation of a geometric action: **composing transformations in sequence**.
- Understanding this helps us see why its properties (like being non-commutative) make perfect sense.

---

### 5. Worked Example: Proving $FR \neq RF$

Let's prove that matrix multiplication is not commutative with a concrete example.

#### Initial Setup

Let's define two simple transformations:

- **Transformation R ( $90^\circ$  Counter-Clockwise Rotation):**
  - $\hat{i}$  becomes  $[0, 1]$
  - $\hat{j}$  becomes  $[-1, 0]$
  - Matrix  $R = \begin{bmatrix} 0 & -1 \\ 1 & 0 \end{bmatrix}$

- **Transformation F (Horizontal Flip / Mirror):**

- $\hat{i}$  becomes  $[1, 0]$  (stays the same)
- $\hat{j}$  becomes  $[0, -1]$  (flips down)
- Matrix  $F = \begin{bmatrix} 1 & 0 \\ 0 & -1 \end{bmatrix}$

We will investigate the difference between  $F * R$  (rotate first, then flip) and  $R * F$  (flip first, then rotate).

---

## Case 1: $F * R$ (Rotate First, then Flip)

### Method #1: Geometric (Following the Basis Vectors)


1. **Start:**  $\hat{i} = [1, 0]$ ,  $\hat{j} = [0, 1]$ .
2. **Step 1 (Apply R):**
  - $\hat{i}$  is rotated  $90^\circ$  to become  $\hat{i}' = [0, 1]$ .
  - $\hat{j}$  is rotated  $90^\circ$  to become  $\hat{j}' = [-1, 0]$ .
3. **Step 2 (Apply F to the RESULT):**
  - We flip  $\hat{i}' = [0, 1]$  horizontally. This flips the y-component:  $\hat{i}'' = [0, -1]$ .
  - We flip  $\hat{j}' = [-1, 0]$  horizontally. This flips the y-component, but it's 0, so it stays:  $\hat{j}'' = [-1, 0]$ .
4. **Resulting Matrix:** The columns are  $\hat{i}''$  and  $\hat{j}''$ .

$$FR = \begin{bmatrix} 0 & -1 \\ -1 & 0 \end{bmatrix}$$

### Method #2: Algebraic (Matrix Multiplication)

$$FR = \begin{bmatrix} 1 & 0 \\ 0 & -1 \end{bmatrix} \begin{bmatrix} 0 & -1 \\ 1 & 0 \end{bmatrix}$$

- **Entry (1,1):** (Row 1 of F)  $\cdot$  (Col 1 of R) =  $[1, 0] \cdot [0, 1] = (1 \cdot 0) + (0 \cdot 1) = 0$ .
- **Entry (1,2):** (Row 1 of F)  $\cdot$  (Col 2 of R) =  $[1, 0] \cdot [-1, 0] = (1 \cdot -1) + (0 \cdot 0) = -1$ .
- **Entry (2,1):** (Row 2 of F)  $\cdot$  (Col 1 of R) =  $[0, -1] \cdot [0, 1] = (0 \cdot 0) + (-1 \cdot 1) = -1$ .
- **Entry (2,2):** (Row 2 of F)  $\cdot$  (Col 2 of R) =  $[0, -1] \cdot [-1, 0] = (0 \cdot -1) + (-1 \cdot 0) = 0$ .
- **Resulting Matrix:**  $\begin{bmatrix} 0 & -1 \\ -1 & 0 \end{bmatrix}$ .

Both methods give the same result! 

---

## Case 2: $R * F$ (Flip First, then Rotate)

## Method #1: Geometric (Following the Basis Vectors)

1. **Start:**  $\hat{i} = [1, 0]$ ,  $\hat{j} = [0, 1]$ .
2. **Step 1 (Apply F):**
  - $\hat{i}$  is flipped to become  $\hat{i}' = [1, 0]$ .
  - $\hat{j}$  is flipped to become  $\hat{j}' = [0, -1]$ .
3. **Step 2 (Apply R to the RESULT):**
  - We rotate  $\hat{i}' = [1, 0]$  by  $90^\circ$ . It moves to the y-axis:  $\hat{i}'' = [0, 1]$ .
  - We rotate  $\hat{j}' = [0, -1]$  by  $90^\circ$ . It moves to the positive x-axis:  $\hat{j}'' = [1, 0]$ .
4. **Resulting Matrix:** The columns are  $\hat{i}''$  and  $\hat{j}''$ .

$$RF = \begin{bmatrix} 0 & 1 \\ 1 & 0 \end{bmatrix}$$

## Method #2: Algebraic (Matrix Multiplication)

$$RF = \begin{bmatrix} 0 & -1 \\ 1 & 0 \end{bmatrix} \begin{bmatrix} 1 & 0 \\ 0 & -1 \end{bmatrix}$$

- **Entry (1,1):**  $[0, -1] \cdot [1, 0] = 0$ .
- **Entry (1,2):**  $[0, -1] \cdot [0, -1] = 1$ .
- **Entry (2,1):**  $[1, 0] \cdot [1, 0] = 1$ .
- **Entry (2,2):**  $[1, 0] \cdot [0, -1] = 0$ .
- **Resulting Matrix:**  $\begin{bmatrix} 0 & 1 \\ 1 & 0 \end{bmatrix}$ .

Both methods give the same result! ✓

---

## Conclusion

Compare our two final results:

- $F * R = \begin{bmatrix} 0 & -1 \\ -1 & 0 \end{bmatrix}$  (This is a reflection across the line  $y=-x$ ).
- $R * F = \begin{bmatrix} 0 & 1 \\ 1 & 0 \end{bmatrix}$  (This is a reflection across the line  $y=x$ ).

The results are completely different. This proves concretely that the order of matrix multiplication matters:  $FR \neq RF$ .

---

## 6. Practice Problems

### Problem 1: Standard Multiplication

Calculate  $A \cdot B$  where:

$$A = \begin{bmatrix} 1 & 2 \\ 3 & 4 \end{bmatrix}, \quad B = \begin{bmatrix} 5 & 6 \\ 7 & 8 \end{bmatrix}$$

**Solution:**

$$A \cdot B = \begin{bmatrix} ? & ? \\ ? & ? \end{bmatrix}$$

- **(1,1):**  $[1, 2] \cdot [5, 7] = (1 \cdot 5) + (2 \cdot 7) = 5 + 14 = 19$
- **(1,2):**  $[1, 2] \cdot [6, 8] = (1 \cdot 6) + (2 \cdot 8) = 6 + 16 = 22$
- **(2,1):**  $[3, 4] \cdot [5, 7] = (3 \cdot 5) + (4 \cdot 7) = 15 + 28 = 43$
- **(2,2):**  $[3, 4] \cdot [6, 8] = (3 \cdot 6) + (4 \cdot 8) = 18 + 32 = 50$

**Answer:**

$$A \cdot B = \begin{bmatrix} 19 & 22 \\ 43 & 50 \end{bmatrix}$$

---

## Problem 2: Composition (Scaling then Shear)

Calculate  $S \cdot T$  where  $S$  is a Shear and  $T$  is a Scaling transformation.

$$S = \begin{bmatrix} 1 & 1 \\ 0 & 1 \end{bmatrix}, \quad T = \begin{bmatrix} 2 & 0 \\ 0 & 3 \end{bmatrix}$$

*Meaning: Apply Scaling first, then apply Shear.*

**Solution:**

$$S \cdot T = \begin{bmatrix} ? & ? \\ ? & ? \end{bmatrix}$$

- **(1,1):**  $[1, 1] \cdot [2, 0] = (1 \cdot 2) + (1 \cdot 0) = 2$
- **(1,2):**  $[1, 1] \cdot [0, 3] = (1 \cdot 0) + (1 \cdot 3) = 3$
- **(2,1):**  $[0, 1] \cdot [2, 0] = (0 \cdot 2) + (1 \cdot 0) = 0$
- **(2,2):**  $[0, 1] \cdot [0, 3] = (0 \cdot 0) + (1 \cdot 3) = 3$

**Answer:**

$$S \cdot T = \begin{bmatrix} 2 & 3 \\ 0 & 3 \end{bmatrix}$$

---

## Problem 3 (Challenge): Reverse Order

Calculate  $T \cdot S$  from the previous problem. Is the result the same?

$$T \cdot S = \begin{bmatrix} 2 & 0 \\ 0 & 3 \end{bmatrix} \begin{bmatrix} 1 & 1 \\ 0 & 1 \end{bmatrix}$$

**Solution:**

$$T \cdot S = \begin{bmatrix} ? & ? \\ ? & ? \end{bmatrix}$$

- **(1,1):**  $[2, 0] \cdot [1, 0] = (2 \cdot 1) + (0 \cdot 0) = 2$
- **(1,2):**  $[2, 0] \cdot [1, 1] = (2 \cdot 1) + (0 \cdot 1) = 2$
- **(2,1):**  $[0, 3] \cdot [1, 0] = (0 \cdot 1) + (3 \cdot 0) = 0$
- **(2,2):**  $[0, 3] \cdot [1, 1] = (0 \cdot 1) + (3 \cdot 1) = 3$

**Answer:**

$$T \cdot S = \begin{bmatrix} 2 & 2 \\ 0 & 3 \end{bmatrix}$$

**Conclusion:**  $S \cdot T \neq T \cdot S$ . This proves again that order matters.

---

## Problem 4 (Non-Square Matrices)

Calculate  $M \cdot N$  where  $M$  is a 2x3 matrix and  $N$  is a 3x2 matrix.

$$M = \begin{bmatrix} 1 & 2 & 3 \\ 4 & 5 & 6 \end{bmatrix}, \quad N = \begin{bmatrix} 7 & 8 \\ 9 & 1 \\ 2 & 3 \end{bmatrix}$$

*(The result will be a 2x2 matrix)*

**Solution:**

$$M \cdot N = \begin{bmatrix} ? & ? \\ ? & ? \end{bmatrix}$$

- **(1,1):**  $[1, 2, 3] \cdot [7, 9, 2] = (1 \cdot 7) + (2 \cdot 9) + (3 \cdot 2) = 7 + 18 + 6 = 31$
- **(1,2):**  $[1, 2, 3] \cdot [8, 1, 3] = (1 \cdot 8) + (2 \cdot 1) + (3 \cdot 3) = 8 + 2 + 9 = 19$
- **(2,1):**  $[4, 5, 6] \cdot [7, 9, 2] = (4 \cdot 7) + (5 \cdot 9) + (6 \cdot 2) = 28 + 45 + 12 = 85$
- **(2,2):**  $[4, 5, 6] \cdot [8, 1, 3] = (4 \cdot 8) + (5 \cdot 1) + (6 \cdot 3) = 32 + 5 + 18 = 55$

**Answer:**

$$M \cdot N = \begin{bmatrix} 31 & 19 \\ 85 & 55 \end{bmatrix}$$

## CONTOH PERKALIAN MATRIKS

$$\begin{bmatrix} 1 & 2 & 3 \\ 4 & 0 & 1 \end{bmatrix} \cdot \begin{bmatrix} 1 & 2 \\ 3 & 1 \\ -1 & 2 \end{bmatrix} =$$

$$\begin{bmatrix} 1.1 + 2.3 + 3.(-1) & 1.2 + 2.1 + 3.2 \\ 4.1 + 0.3 + 1.(-1) & 4.2 + 0.1 + 1.2 \end{bmatrix} =$$

$$\begin{bmatrix} 4 & 10 \\ 3 & 10 \end{bmatrix}$$

$$\begin{bmatrix} 4 & 5 \\ 2 & 6 \end{bmatrix} \times \begin{bmatrix} 1 & 2 \\ 3 & 4 \end{bmatrix}$$

$$= \begin{bmatrix} (4 \times 1) + (5 \times 3) & (4 \times 2) + (5 \times 4) \\ (2 \times 1) + (6 \times 3) & (2 \times 2) + (6 \times 4) \end{bmatrix}$$

$$= \begin{bmatrix} 4 + 15 & 8 + 20 \\ 2 + 18 & 4 + 24 \end{bmatrix}$$

$$= \begin{bmatrix} 19 & 28 \\ 20 & 28 \end{bmatrix}$$

**Tags:** #mml-special-ization #linear-algebra #matrix-multiplication #compositions  
#transformations